\subsection*{Deductive proof of the tetrahedral number formula}
\subsubsection*{Proof}

%\begin{proof}

%\end{proof}

\begin{enumerate}
	\item Let $g(n)$ be the $n$th triangular number.

		$g(n) = \frac{n(n+1)}{2}$
	\item Let $F(n)$ be the $n$th tetrahedral number.
	
		$F(n) = \sum\limits_{i=1}^n g(i)$
	\item Substitute:
		
		$F(n) = \sum\limits_{i=1}^n \frac{i(i+1)}{2}$
	\item Distribute:
	
		$F(n) = \sum\limits_{i=1}^n \frac{i^2}{2} + \frac{i}{2}$
	\item Split:
	
		$F(n) = \sum\limits_{i=1}^n \frac{i^2}{2} + \sum\limits_{i=1}^n \frac{i}{2}$
	\item Take out constants:
	
		$F(n) = \frac{1}{2} \sum\limits_{i=1}^n i^2 + \frac{1}{2} \sum\limits_{i=1}^n i$
	\item Substitute known formulas for sums:
	
		$F(n) = \frac{1}{2} \left( \frac{n(n+1)(2n+1)}{6} + \frac{n(n+1)}{2} \right) $
	\item Add:
	
		$F(n) = \frac{1}{2} \left( \frac{n(n+1)(2n+1) + 3n(n+1)}{6} \right) $
	\item Factor:
	
		$F(n) = \frac{1}{2} \left( \frac{n(n+1) ((2n+1) + 3))}{6} \right) $
	\item Simplify:
	
		$F(n) = \frac{1}{2} \left( \frac{n(n+1) (2n+4 )}{6} \right) $
	\item Simplify:
	
		$F(n) = \frac{1}{2} \left( \frac{2n(n+1) (n+2 )}{6} \right) $

\end{enumerate}

\begin{center}$\therefore F(n) = \frac{n(n+1)(n+2)}{6}$ \end{center}
